\input{header}
\input{macros}
\sheet{5}{November 22nd, 2024}
\usepackage{algorithm}
\usepackage[noend]{algpseudocode}
\begin{document}
\setcounter{section}{1}

\section{Syntactical sugar}

\subsection{(a)}

Statement: \( x_i := x_j^{x_k} \)

\begin{algorithmic}[1]
\State \( x_i := 1; \)
\For{\( x_k \)}
    \State \( x := 0; \)
    \For{\( x_j \)}
        \State \( x := x + x_i; \)
    \EndFor \textbf{od;}
    \State \( x_i := x; \)
\EndFor \textbf{od;}
\end{algorithmic}


\subsection{(b)}

\begin{algorithmic}[1]
\State \( x_{cmp} := 1; \)  
\For{\( x_i \)}
    \State \( x_{cmp} := 0; \) 
\EndFor \textbf{od;}
\For{\( x_{cmp} \)}
     \( P_1; \)
\EndFor \textbf{od;}
\For{\( x_i \)}
    \State\( P_2; \)
\EndFor \textbf{od;}
\end{algorithmic}


\subsection{(c)}

\begin{algorithmic}[1]
\State \( x_i := 0; \)
\For{\( x_j \)}
    \If{\( x_j \geq x_k \)}
        \State \( x_j := x_j - x_k; \)
        \State \( x_i++; \)
    \Else
        \State \(x_i := x_i;\)
    \EndIf
\EndFor \textbf{od;}
\end{algorithmic}

\subsection{(d)}

\begin{algorithmic}[1]

\For{\( x_j \)}
    \If{\( x_j \geq x_k \)}
        \State \( x_j := x_j - x_k; \)
    \Else
        \State \textbf{break;}
    \EndIf
\EndFor \textbf{od;}
\State \( x_i := x_j; \) 
\end{algorithmic}


\subsection*{(e) Generalized Conditional Statements}

We can reuse the program from (b) to implement this statement by first simulating \( x_i \circ x_j \) and setting an auxiliary variable \( x_k \) to \( 0 \) if \( x_i \circ x_j \) is true, and \( 1 \) otherwise.
\subsubsection*{Simulating \( = \):}
\begin{algorithmic}[1]
\State \( x_k := x_i - x_j; \)
\If{\( x_k = 0 \)}
    \State  \( P_1; \)
\Else
    \State  \( P_2; \)
\EndIf \textbf{fi;}
\end{algorithmic}

\subsubsection*{Simulating \(  \neq \):}
\begin{algorithmic}[1]
\State \( x_k := x_i - x_j; \)
\State \( x_t := 1; \)
\For{\( x_k \)}
    \State \( x_t := 0; \)
\EndFor \textbf{od;}
\If{\( x_t = 0 \)}
    \State  \( P_1; \)
\Else
    \State  \( P_2; \)
\EndIf \textbf{fi;}
\end{algorithmic}

\subsubsection*{Simulating \(  \geq \):}
\begin{algorithmic}[1]
\State \( x_k := x_j - x_i; \)
\If{\( x_k = 0 \)}
    \State  \( P_1; \)
\Else
    \State  \( P_2; \)
\EndIf \textbf{fi;}
\end{algorithmic}

\subsubsection*{Simulating \(  > \):}
\begin{algorithmic}[1]
\State \( x_k := x_i - x_j; \)
\State \( x_t := 1; \)
\For{\( x_k \)}
    \State \( x_t := 0; \)
\EndFor \textbf{od;}
\If{\( x_t = 0 \)}
    \State  \( P_1; \)
\Else
    \State  \( P_2; \)
\EndIf \textbf{fi;}
\end{algorithmic}

\subsubsection*{Simulating \(  < \):}
\begin{algorithmic}[1]
\State \( x_k := x_j - x_i; \)
\State \( x_t := 1; \)
\For{\( x_k \)}
    \State \( x_t := 0; \)
\EndFor \textbf{od;}
\If{\( x_t = 0 \)}
    \State  \( P_1; \)
\Else
    \State  \( P_2; \)
\EndIf \textbf{fi;}
\end{algorithmic}

\subsubsection*{Simulating \( \leq \):}
\begin{algorithmic}[1]
\State \( x_k := x_i - x_j; \)
\If{\( x_k = 0 \)}
    \State  \( P_1; \)
\Else
    \State  \( P_2; \)
\EndIf \textbf{fi;}
\end{algorithmic}


\end{document}
