\input{header}
\input{macros}
\sheet{6}{November 29th, 2024}
\begin{document}

\section{Transducers}
a)

Automata recognizing \( f_N(K) \):

\begin{tikzpicture}[shorten >=1pt, node distance=3cm, on grid, auto] 
   \node[state, initial] (SS') {$SS'$}; 
   \node[state] (XA') [right=of SS'] {$XA'$}; 
   \node[state] (XA'_0) [right=of XA'] {$XA'_0$}; 
   \node[state] (AS') [right=of XA'_0] {$AS'$};
   \node[state] (SA') [below=of SS'] {$SA'$}; 
   \node[state] (XS') [right=of SA'] {$XS'$}; 
   \node[state] (XS'_0) [right=of XS'] {$XS'_0$}; 
   \node[state, accepting] (AA') [right=of XS'_0] {$AA'$};

   \path[->] 
    (SS') 
          edge [bend right] node {$\varepsilon$} (SA')
          edge [bend right] node {1} (XA')
    (XA') edge node {1} (XA'_0)
          edge [bend right] node {1} (SS')
    (XA'_0) edge node {0} (AS')
    (AS') edge [bend right] node {$\varepsilon, 0$} (AA')
    (SA') 
          edge [bend right] node {1} (XS')
          edge [bend right] node {$\varepsilon$} (SS')
    (XS') edge node {1} (XS'_0)
          edge [bend right] node {1} (SA')
    (XS'_0) edge node {0} (AA')
    (AA') edge [pos=0.25, bend right] node {$\varepsilon, 0$} (AS');
\end{tikzpicture}

Automata recognizing \( f_N^{-1}(K) \):

\begin{tikzpicture}[shorten >=1pt, node distance=3cm, on grid, auto] 
   \node[state, initial] (SS') {$SS'$}; 
   \node[state] (XA') [right=of SS'] {$XA'$}; 
   \node[state, accepting] (AA') [right=of XA'] {$AA'$};
   \node[state] (AS') [right=of XS'] {$AS'$};

   \path[->] 
    (SS') edge [loop above] node {1} (SS')
          edge [bend right] node {0} (XA')
    (XA') edge node {0} (AA')
          edge [bend right] node {1} (SS')
    (AA') edge [loop above] node {0} (AA')
          edge [bend right] node {1} (AS')
    
    (AS') edge [loop below] node {0} (AS')
          edge [bend right] node {1} (AA');
\end{tikzpicture}

\textbf{b)} Let $M_L = (Q_L, \Sigma, \delta_L, q_0, Q_{\text{acc},L})$ be a DFA with $L = L(M_L)$.

We construct an NFA $M_{f_M} = (Q_{f_M}, \Gamma, \delta_{f_M}, (q_0, q_{0, L}), Q_{\text{acc},f_M})$, s.t. $f_M(L) = L(L(M_{f_M}))$.

\[
Q_{f_M} = (Q \times Q_L) \cup \{(q, q_L)_{f(q,a)_i} \mid q \in Q, q_L \in Q_L, a \in \Sigma, 1 \leq i \leq |f(q, a)|\}
\]

\[
Q_{\text{acc},f_M} = \{(q, q_L) \mid q \in Q_{\text{acc}} \land q_L \in Q_{\text{acc},L}\}.
\]

To formally define the set of $\delta$ transitions, we will interpret $\delta_{f_M}$ as a \emph{set of triplets} as follows:

\[
((q, q_L), a, (q', q_L')) \in \delta_{f_M} \iff (q', q_L'), a) \in \delta_{f_M}((q, q_L), a).
\]

Similar to sample solution 2, in particular, we have:
\[
\delta_{f_M} :=
\{((q, a, q_L), f(q, a), (q', q_L')) \mid |f(q, a)| \leq 1, (q, a, q') \in \delta, (q_L, a, q_L') \in \delta_L\}
\]
\[
\cup \{((q, q_L), f(q, a)_1, (q', q_1')_{f(q, a)_1}) \mid |f(q, a)| > 1, (q, a, q') \in \delta, (q_L, a, q_L') \in \delta_L\}
\]
\[
\cup \{((q, q_L)_{f(q, a)_i}, f(q, a)_{i+1}, (q', q_L')_{f(q, a)_{i+1}}) \mid 1 \leq i \leq |f(q, a)| - 2, (q, a, q') \in \delta, (q_L, a, q_L') \in \delta_L\}
\]
\[
\cup \{((q, q_L)_{f(q, a)_{|f(q, a)|-1}}, f(q, a)_{|f(q, a)|}, (q', q_L')) \mid  (q_L, a, q_L') \in \delta_L, |f(q, a)| > 1\}
\]
This way, $\delta_{f_M}$ handles all the cases, including the transitions to and from the artificial states. This is what the three last subsets of $\delta_{f_M}$ handle.

Note that these artificial states are being introduced due to the fact that in $f(q, a) = b$, $a \in \Sigma$ but $b \in \Gamma^*$, which we need to traverse.

\noindent
\textbf{(c)}
Let $M_L = (Q_L, \Gamma, \delta_L, q_0, Q_{\text{acc},L})$ such that $L = L(M_L)$.

We construct a DFA $M_{f_M^{-1}} = ((Q \times Q_L), \Sigma, \delta_{f_M^{-1}}, (q_0, q_0), Q_{\text{acc},f_M^{-1}})$ with:

\[
Q_{\text{acc},f_M^{-1}} = \{(q, q_L) \mid q \in Q_{\text{acc}} \land q_L \in Q_{\text{acc},L} \}
\]

and

\[
\delta_{f_M^{-1}}((q, q_L), \sigma) =
\begin{cases} 
  (\delta(q, a), \delta_L^*(q_L, f(q, a))) & \text{if } \delta(q, a) \in Q \\
  & \land \delta_L^*(q_L, f(q, a)) \in Q_L \\
  & \land f(q, a) \text{ is defined} \\
  \text{undefined} & \text{otherwise.}
\end{cases}
\]

Now this automaton recognizes $f_M^{-1}$ such that $f_M^{-1}(L) = L(M_{f_M}^{-1})$.



\noindent
\textbf{(d)} If \( h: \Sigma^* \to \Gamma^* \) is a homomorphism, then there is a transducer \( M \) with \( f_M = h \).

Let \( h: \Sigma^* \to \Gamma^* \) be a homomorphism.  
We can construct a transducer as follows:

\[
\sigma \in \Sigma: h(\sigma)
\]

Formally, 
\[
M_h = (Q, \Sigma, \Gamma, \delta, f, q_0, Q_{\text{acc}})
\]
with
\[
Q = \{ q_0 \}, \quad Q_{\text{acc}} = \{ q_0 \},
\]
\[
\delta(q_0, x) = q_0, \quad \forall x \in \Sigma^*,
\]
and
\[
f^*(q_0, x) = h(x).
\]

Now, we prove that \( \forall x \in \Sigma^* : f^*(q_0, x) = h(x) \).

Proof by induction over \( |x| \):  

\textbf{Base case:}  
If \( |x| = 0 \), \( x = \varepsilon \):  
\[
f^*(q_0, \varepsilon) = h(\varepsilon) = \varepsilon.
\]

\textbf{Induction step:}  
Let \( |w| = n + 1 \), where \( w = \sigma x \), \( x \in \Sigma^* \), and \( \sigma \in \Sigma \).

Induction Hypothesis (IH): Assume \( f^*(q_0, x) = h(x) \) for all \( x \in \Sigma^* \) with \( |x| = n \).  
We prove it holds for \( w = \sigma x \):  

\[
f^*(q_0, w) = f^*(q_0, \sigma x)
\]
\[
= f(q_0, \sigma) f^*(q_0, x)
\]
\[
= h(\sigma) h(x)
\]
\[
= h(\sigma x)
\]
\[
= h(w).
\]

Thus, by induction, \( f^*(q_0, x) = h(x) \) for all \( x \in \Sigma^* \). \(\Box\)

\begin{itemize}
    \item[(e)] Yes, for example:
\end{itemize}
\begin{center}
\begin{tikzpicture}[shorten >=1pt, node distance=2cm, on grid, auto]
   \node[state, initial] (s)   {$S$}; 
   \node[state] (s') [right=of s] {$S'$}; 
    \path[->] 
    (s) 
        edge [bend left] node {1:1} (s')
    (s') 
        edge [bend left] node {1:0} (s);
\end{tikzpicture}
\end{center}

It holds that $f_M(11) = 10 \neq 11 = f_M(1)f_M(1)$.

This shows that $f_M$ does not have the property of a homomorphism.


\end{document}
